\documentclass[UTF8,a4paper,12pt,scheme=chinese]{ctexart}

\setlength{\textwidth}{550pt}
\setlength{\hoffset}{-1.2in}
\setlength{\voffset}{-1in}

\usepackage{amsmath}
\usepackage{textcomp} 
\usepackage{graphicx}
\usepackage{xcolor}

\newcommand{\hlx}[2]{%
	\IfEqCase{#1}{%
		{1}{
			\colorbox{yellow!50}{$\displaystyle#2$}
		}
		{b}{
			\colorbox{yellow!50}{$\scriptstyle#2$}
		}
		{3}{
			\colorbox{yellow!50}{$\scriptscriptstyle#2$}
		}
	}
		% you can add more cases here as desired
	
}%


\pagestyle{headings}
\ctexset{section={
		name={第,章},
		number=\arabic{section},
	},
subsection={
	name={第,节},
	number=\arabic{subsection},
},
}


\newcommand{\ud}{\mathrm{d}}
\newcommand{\lc}{\left(}
\newcommand{\rc}{\right)}

\newcommand{\hl}[1]{\colorbox{yellow}{#1}}
\newcommand{\hla}[1]{%
	\colorbox{yellow!50}{$\displaystyle#1$}}
\newcommand{\hlb}[1]{%
	\colorbox{yellow!50}{$\scriptstyle#1$}}
\newcommand{\hlc}[1]{%
	\colorbox{yellow!50}{$\scriptscriptstyle#1$}}

\makeatletter
\DeclareFontFamily{U}{tipa}{}
\DeclareFontShape{U}{tipa}{m}{n}{<->tipa10}{}
\newcommand{\arc@char}{{\usefont{U}{tipa}{m}{n}\symbol{62}}}%

\newcommand{\arc}[1]{\mathpalette\arc@arc{#1}}

\newcommand{\arc@arc}[2]{%
	\sbox0{$\m@th#1#2$}%
	\vbox{
		\hbox{\resizebox{\wd0}{\height}{\arc@char}}
		\nointerlineskip
		\box0
	}%
}
\makeatother

\begin{document}
	\begin{Large}
		\begin{enumerate}
			\item $\frac{\sin n \alpha}{n^4}$
			\item 定理8$|u_n| 收敛 \rightarrow u_n 收敛 $
			\item $(-1)^n\frac{n^2}{e^n}$
			\item $\frac{\cos x}{n^3}$
			\item $(-1)^{n+1}\frac{1}{\sqrt{n+1}}$
			\item $(-1)^n\frac{\ln n}{n}$
			
			\item $(-1)^{n-1}\frac{1}{n^p}$
			\item $(-1)^n\frac{k+n}{n^2}$
			\item $(-1)^n\frac{n^{n+1}}{(n+1)!}$
			\item $(-1)^n\frac{1}{n-\ln n}$
			
			\item $\frac{(-1)^n}{2^n}\left(1+\frac{1}{n}\right)^{n^2}$
			\item $(-1)^n(\sqrt{n-1}-\sqrt{n})$
			\item $(-1)^n\ln(\frac{n+1}{n})$
			\item $\frac{n^{n+\frac{1}{n}}}{\left(n+\frac{1}{n}\right)^n}$
			
			\item $\frac{3^n}{n!2^n}$
			\item $\frac{\ln(n+2)}{(a+\frac{1}{n})^n}$
			\item $\frac{a^n}{n^p}$（p大于0,a为常数）
			\item $\frac{a^n}{1+a^{2n}}$（a为常数）
		\end{enumerate}
		\begin{enumerate}
			\item $\left(|u_n| \rightarrow\times 0 \right)\rightarrow \left(u_n \rightarrow\times 0\right)$
		\end{enumerate}
		\begin{enumerate}
			\item $\frac{1}{n^n}$
			\item $\frac{2+(-1)^n}{2^n}$
			\item $\frac{1}{\ln(n+1)}$
			\item $\frac{2n+1}{(n+1)^2(n+2)^2}$
			\item $\frac{3^n}{1+e^n}$
			\item $\frac{(n!)^2}{(2n)!}$
			\item $\frac{n^2}{\left(2+\frac{1}{n}\right)^n}$
			\item $\frac{1}{3^n}\left(2+\frac{1}{n}\right)^n$
			\item $\frac{a^{n-1}}{1+a^n}$（a大于0）
			\item
			\item $(-1)^{n-1}\frac{1}{n}$，
			$(-1)^{n-1}\frac{1}{n!}$，
			$(-1)^{n-1}\frac{n}{10^n}$
			\item $\sum_{n=2}^{\infty}(-1)^n\frac{1}{\ln n}$
			\item $\sum_{n=2}^{\infty}(-1)^n\frac{\sqrt{n}}{n-1}$
			\item $(-1)^n\frac{\ln n}{n}$
			\item $(-1)^n\frac{1}{n-\ln n}$
			\item $(-1)^n\frac{1}{\sqrt{n}+(-1)^n}$
			\item $(-1)^n\frac{1}{\sqrt{n+(-1)^n}}$
		\end{enumerate}
		\begin{enumerate}
			\item $\frac{1}{n(2n+1)}$
			\item $\frac{n\cos^2\frac{n\pi}{3}}{(n+1)^3}$
			\item $\frac{n}{(n+1)(n+3)}$
			\item $\arcsin\frac{2}{n}$
			\item $1-\cos\frac{2}{n}$
			\item $\ln(1+\frac{2}{n^2})$
			\item $\frac{n!}{a^n}$（a大于0）
			\item $\frac{(2n)!}{n!3^n}$
			\item $\frac{3^{2n}}{n^2}$
			\item $\left(\sqrt{\frac{n-1}{9n+1}}\right)^n$
			\item $\left(\frac{n}{2n-1}\right)^{2n-1}$
		\end{enumerate}
		\begin{enumerate}
			\item $n\sin\frac{\pi}{4^n}$
			\item $\frac{n^{n+1}}{(n+1)!}$
			\item $2^n\frac{n!}{(2n)!}$
			\item $\frac{(4n+1)!}{4^nn^4}$
			\item $\frac{1}{n\sqrt{n+1}}$
			\item $2^n\ln(1+\frac{1}{3^n})$
			\item $\frac{n!}{(2n)!}\sin\frac{1}{4^n}$
		\end{enumerate}
		\begin{enumerate}
			\item 	$ (-1)^n\dfrac{1}{\ln(2+n)} $
			\item 	$ (-1)^{n-1}\dfrac{n}{4^n} $
			\item 	$ \dfrac{\sin\dfrac{a}{n+1}}{a^{n+1}}(a>1) $
			\item 	$ (-1)^n\dfrac{\sin\sqrt{n}}{n^2} $
			\item 	$ \dfrac{\cos n \pi}{n+1} $
			\item 	$ (-1)\sin\dfrac{x}{n} $
			\item 	$ (-1)^n\dfrac{\ln n}{n^p}(0<p\leq1) $
			\item 	$ \dfrac{1}{\sqrt{n}}\cos\dfrac{n\pi}{2} $
			\item 	$ \dfrac{1}{\sqrt{n}}\sin\dfrac{n\pi}{2} $
			\item 	$ \dfrac{(-1)^n}{\ln^2(n+1)}(\sin\dfrac{1}{n}) $
			\item 	$ u_n $收敛，$ \dfrac{u_n}{n^{1+a}} $绝对收敛？
			\item 	$ a_n $收敛，$ b_n $条件收敛，$ a_n-b_n $条件收敛?
			\item 	$ n^2x^n $
			\item 	$ \dfrac{nx^n}{(2n)!!} $
			\item 	$ (-1)^n\dfrac{x^n}{n\cdot4^n} $
			\item 	$ \dfrac{2+n}{1+n^2}(2x-5)^n $
			\item 	$ (1+\dfrac{2}{n})^{-n^2}x^n $
			\item 	$ a^{n^2}x^n(a>0) $
			\item 	$ \dfrac{x^n}{1+x^{2n}} $
			\item 	$ (1+\dfrac{1}{n})^{n^2}x^n $
			\item	$ \dfrac{(n!)^2}{(2n)!}x^n $
			\item 	$  $
			\item 	$  $
			\item 	$  $
			\item 	$ nx^n $
			\item 	$ \dfrac{x^n}{x+1} $
			\item 	$ (-1)^{n-1}\dfrac{x^n}{n} $
			\item 	$ n(n+1)x^n $
			\item 	$ \dfrac{x^{2n+1}}{(2n+1)!} $
			\item 	$ f(x)=e^x $
			\item 	$ f(x)=\sin x $
			\item 	$ f(x)=\dfrac{x^{4n+1}}{4n+1} $
			\item 	$ \dfrac{1}{1+x^2},x $
			\item 	$ \arctan x,x $
			\item 	$ \sin x,x-\dfrac{\pi}{4} $
			\item 	$ \dfrac{1}{3-x},x,x-1 $
			\item 	$ \dfrac{1}{x^2+4x+3},x-1 $
			\item 	$ f(x)=\sin x \cos 2x $
			\item 	$ \ln(1+x-2x^2),x $
			\item 	$ \dfrac{1}{x^2-5x+6} $
			\item 	$ \dfrac{x-1}{4-x},(x-1),f^{(n)}(1) $
			\item 	$ sin^2x,x $
			\item 	$ f(x)=\left\lbrace \begin{array}{ll}-1,&-\pi\leq x{<}0\\1,&0{<}x\leq\pi\end{array} \right. $
			\item 	$ f(x)=\left\lbrace \begin{array}{ll}x,&-\pi\leq x{<}0\\0,&0{<}x\leq\pi\end{array} \right. $
			\item 	$ f(x)=\left\lbrace \begin{array}{ll}-x,&-\pi\leq x{<}0\\x,&0{<}x\leq\pi\end{array} \right. $
			\item 	$ f(x)=x+1, $正弦，余弦
			\item 	$ f(x)=\left\lbrace \begin{array}{ll}x,&2{<}|x|\leq\pi\\x,&|x|\leq2\end{array} \right. $
			\item 	$ f(x)=\left\lbrace \begin{array}{ll}\pi x+x^2,&-\pi\leq x{<}0\\\pi x-x^2,&0\leq x{<}\pi\end{array} \right. $
			\item 	证明
			\item 	空
			\item 	$ \dfrac{1}{n\sqrt[n]{n}} $	发散
			\item 	$ \dfrac{(n!)^2}{2n^2} $	发散
			\item 	$ \dfrac{n\cos^2\dfrac{n\pi}{3}}{2^n} $	收敛
			\item 	$ \dfrac{1}{(\ln n)^10} $	发散
			\item 	证明.正项$n=1 u_n $收敛，$n=1 v_n $收敛，$ (u_n+v_n)^2 $收敛?	收敛
			\item 	证明.非正项$n=1 u_n $收敛，$\lim\limits_{n\rightarrow \infty}\dfrac{v_n}{u_n}=1$收敛，$ v_n $收敛?	发散
			\item 	$ (-1)^n\dfrac{1}{n^p},p $为常数	绝对收敛
			\item 	$ (-1)^{n+1}\dfrac{sin\dfrac{\pi}{n+1}}{\pi^{n+1}} $	绝对收敛
			\item 	$ (-1)\ln\dfrac{n+1}{n} $	没做
			\item 	$ (-1)^n\dfrac{(n+1)!}{n^{n+1}} $	收敛
			\item 	$ \lim\limits_{n\rightarrow \infty}\dfrac{1}{n}\sum_{k=1}^{n}\dfrac{1}{3^k}(1+\dfrac{1}{k})^{k^2} $	0
			\item 	$ \lim\limits_{n\rightarrow \infty}[2^{\dfrac{1}{3}}\cdot{(2^n)}^{\dfrac{1}{3^n}}] $	2
			\item 	$ \dfrac{2n-1}{2^n}x^{2(n-1)} $没有偶项	长
			\item 	$ f(x)=\arctan\dfrac{1+x}{1-x},x $	长
			\item 	$ \dfrac{n^2}{n!} $	长
			\item 	$ f(x)=3x^2+1 $	长
			\item 	$ f(x)=\left\lbrace \begin{array}{ll}bx,&-\pi\leq x{<}0\\ax,&0\leq x{<}\pi\end{array} \right.(a{>}b{>}0) $
			\item 	$ f(x)=\left\lbrace \begin{array}{ll}e^x,&[-\pi,0)\\1,&[0,\pi]\end{array} \right.(a{>}b{>}0) $
			\item 	$ f(x)=\left\lbrace \begin{array}{ll}-\dfrac{\pi}{2},&[-\pi,-\dfrac{\pi}{2})\\x,&[-\dfrac{\pi}{2},-\dfrac{\pi}{2})\\\dfrac{\pi}{2},&[\dfrac{\pi}{2},\pi)\end{array} \right. $
			\item 	$ f(x)=2x^2[0,\pi], $正弦，余弦
			\item 	$ \dfrac{3^n+5^n}{n}x^n $
			\item 	文字表述求微分方程表达式
			\item 	$ \dfrac{\ud y}{\ud x}=\dfrac{1}{2}(y^2-1) $
			\item 	$ (1+y^2)\ud x + y(x+1) \ud y =0 $
			\item 	$ y'=\dfrac{1}{2}\tan^2(x+2y) $
			\item 	$ y'=\sin^2(x-y+1) $
			\item 	$ (x+xy^2)\ud x - (x^2y + y)\ud y =0 $
			\item 	$ y'+\sin(x+y)=\sin(x-y) $
			\item 	$ \dfrac{\ud y}{\ud x}e^{x+y} $
			\item 	$ xy\ud x +(x^2+1)\ud y=0,y(0)=1 $
			\item 	$ \dfrac{\ud y}{\ud x}=\sqrt{ax+by+c} $
			\item 	$ y'=\dfrac{y}{x}+\tan\dfrac{y}{x} $
			\item 	$ (x-y\cos\dfrac{y}{x})\ud x+x\cos\dfrac{y}{x}\ud y =0 $
			\item 	$ \dfrac{\ud x}{x^2-xy+y^2}=\dfrac{\ud y}{2y^2-xy} $
			\item 	$ (1+2e^{\frac{x}{y}})\ud x+2e^{\frac{x}{y}}(1-\dfrac{x}{y})=0 $
			\item 	$ (y^2-2xy)\ud x + x^2\ud y=0 $
			\item 	$ \dfrac{\ud y}{\ud x}=\dfrac{x+y}{x-y} $
			\item 	$ y'+\dfrac{1}{x}y=\dfrac{\sin x}{x} $
			\item 	$ \dfrac{\ud y}{\ud x}-\dfrac{2y}{x+1}=(x+1)^{\frac{5}{2}} $
			\item 	$ (1+x^2)y''+2xy'=1 $
			\item 	$ \dfrac{\ud y}{\ud x}=\dfrac{y}{x+y^3} $
			\item 	$ \dfrac{\ud y}{\ud x}+\dfrac{y}{x}=a(\ln x)y^2 $
		\end{enumerate}
	\end{Large}
\end{document}